Re-implemented do_computation_equal, and completed correctness proof.

reify/do_computation.v
@@ -12,18 +12,18 @@ Require Import MirrorShard.Expr.
 
 Module do_computation (uk : unknown_types).
 
-Module our_funcs := funcs uk.
-Import our_funcs.
-Import all_types.
+  Module our_funcs := funcs uk.
+  Import our_funcs.
+  Import all_types.
 
-(* Cleaner syntax for Nat pattern-matches and function lists *)
-Local Open Scope nat.
-Import List.
-Import ListNotations.
+  (* Cleaner syntax for Nat pattern-matches and function lists *)
+  Local Open Scope nat.
+  Import List.
+  Import ListNotations.
 
-(* Listing of which functions compute directly into consts (taking no arguments)
- * and which do not. *)
-(*
+  (* Listing of which functions compute directly into consts (taking no arguments)
+   * and which do not. *)
+  (*
 Definition is_const_base (f : func) :=
   match f with
     | 1  (* O_f *)
@@ -39,122 +39,99 @@ Definition is_const_base (f : func) :=
       => true
 
     | _ => false
-  end.            
-*)
-Definition is_const_base (f : func) :=
-NPeano.ltb f computable_prefix_length.
+  end.
+   *)
+  Definition is_const_base (f : func) :=
+    NPeano.ltb f computable_prefix_length.
 
-(* Decide if an expression can compute directly into a Const
- * (by converting the pre-defined functions we have defined
- * as convertible into consts) *)
-Fixpoint is_const (e : expr all_types) :=
-  let is_const_l (es : list (expr all_types)) : bool :=
-      fold_right andb true (map is_const es)
-  in
-  match e with
+  (* Decide if an expression can compute directly into a Const
+   * (by converting the pre-defined functions we have defined
+   * as convertible into consts) *)
+  Fixpoint is_const (e : expr all_types) :=
+    let is_const_l (es : list (expr all_types)) : bool :=
+        fold_right andb true (map is_const es)
+    in
+    match e with
       (* it and its arguments must be const *)
-    | Func f es => andb (is_const_base f) (is_const_l es)
-    | Const _ _ => true
-(*    | Equal _ l r => andb (is_const l) (is_const r) *)
-    | _ => false
+      | Func f es => andb (is_const_base f) (is_const_l es)
+      | Const _ _ => true
+      (*    | Equal _ l r => andb (is_const l) (is_const r) *)
+      | _ => false
 
-  end.             
+    end.
 
-(* Simplify an expression, if we can.
- * Expects that a user-supplied Ltac will have already converted
- * user-defined functions into Consts, as appropriate *)
-Definition do_computation (user_functions : list (signature all_types)) (e : expr all_types) (t : tvar) : 
-option (tvarD all_types t) :=
-if is_const e then
-  match (@exprD all_types (functions ++ user_functions) nil nil e t) with
-    | Some v => Some v
-    | None => None (** should be dead code if e is well typed **)
-  end
-else
-  None.
+  (* Simplify an expression, if we can.
+   * Expects that a user-supplied Ltac will have already converted
+   * user-defined functions into Consts, as appropriate *)
+  Definition do_computation (user_functions : list (signature all_types)) (e : expr all_types) (t : tvar) :
+    option (tvarD all_types t) :=
+    if is_const e then
+      match (@exprD all_types (functions ++ user_functions) nil nil e t) with
+        | Some v => Some v
+        | None => None (** should be dead code if e is well typed **)
+      end
+    else
+      None.
 
-Lemma do_computation_correct : forall (user_functions : list (signature all_types)) (e : expr all_types) (t : tvar) (v : tvarD all_types t),
-do_computation user_functions e t = Some v ->
-forall (vars uvars : env all_types),
-exprD (functions ++ user_functions) uvars vars e t = Some v.
-Proof.
-  intros.
-  unfold do_computation in *.
-  destruct (is_const e); try congruence.
-  remember (exprD (functions ++ user_functions) [] [] e t) as exprDf.
-  destruct exprDf.
-  - inversion H; subst.
-    symmetry in HeqexprDf.
-    eapply exprD_weaken in HeqexprDf.
-    eassumption.
-  - inversion H.
-Qed.
+  Lemma do_computation_correct : forall (user_functions : list (signature all_types)) (e : expr all_types) (t : tvar) (v : tvarD all_types t),
+                                   do_computation user_functions e t = Some v ->
+                                   forall (vars uvars : env all_types),
+                                     exprD (functions ++ user_functions) uvars vars e t = Some v.
+  Proof.
+    intros.
+    unfold do_computation in *.
+    destruct (is_const e); try congruence.
+    remember (exprD (functions ++ user_functions) [] [] e t) as exprDf.
+    destruct exprDf.
+    - inversion H; subst.
+      symmetry in HeqexprDf.
+      eapply exprD_weaken in HeqexprDf.
+      eassumption.
+    - inversion H.
+  Qed.
 
-(* Some fun little examples *)
-Eval vm_compute in (do_computation nil (Func 13 [(Func 1 [])]) (tvType 11)).
-Eval vm_compute in (do_computation nil (Equal nat_tv (Func 1 []) (Func 1 [])) tvProp).
-Eval vm_compute in (do_computation nil (Equal nat_tv (Func 13 [(Func 1 [])]) (Func 1 [])) tvProp).
-Eval vm_compute in (do_computation nil (Equal nat_tv (Func 13 [(Func 1 [])]) (Func 13 [(Func 1 [])])) tvProp).
+  (* Some fun little examples *)
+  Eval vm_compute in (do_computation nil (Func 13 [(Func 1 [])]) (tvType 11)).
 
-Print expr.
-Print tvar.
-Check nth_error.
+  Eval vm_compute in (do_computation nil (Equal nat_tv (Func 1 []) (Func 1 [])) tvProp).
+  Eval vm_compute in (do_computation nil (Equal nat_tv (Func 13 [(Func 1 [])]) (Func 1 [])) tvProp).
+  Eval vm_compute in (do_computation nil (Equal nat_tv (Func 13 [(Func 1 [])]) (Func 13 [(Func 1 [])])) tvProp).
+  
+  Definition do_computation_equal (user_functions : list (signature all_types)) (e : expr all_types) : bool :=
+    match e with
+      | Equal t l r =>
+        match do_computation user_functions l t with
+          | Some l' =>
+            match do_computation user_functions r t with
+              | Some r' => get_Eq all_types t l' r'
+              | _ => false
+            end
+          | _ => false
+        end
+      | _ => false
+    end.
 
-Eval vm_compute in (nth_error [1; 2; 3; 4] 3).
-Print Impl.
-Print Sig.
+  (* some tests for do_computation_equal *)
+  Eval vm_compute in (do_computation nil (Func 1 []) (tvType 11)).
+  Eval vm_compute in (do_computation_equal nil (Equal (tvType 11) (Func 13 [(Func 1 [])]) (Func 13 [(Func 1 [])]))).
 
-(* Computes an Expr that represents an equality (for types with decidable equality), 
- * Appealing to the decision procedures contained in the type signature *)
-Check const_seqb.
-Print const_seqb.
-Locate const_seqb.
+  (* consider tactic needed for this correctness proof *)
+  Require Import ExtLib.Tactics.Consider.
+  Lemma do_computation_equal_correct :
+    forall (user_functions : list (signature all_types)) (t : tvar) (l r : expr all_types),
+      do_computation_equal user_functions (Equal t l r) = true ->
+      exists (res : tvarD all_types t),
+        do_computation user_functions l t = Some res /\
+        do_computation user_functions r t = Some res.
 
-
-Definition do_computation_equal (user_functions : list (signature all_types)) (e : expr all_types) : bool.
-remember e as exp; destruct e.
-(* We just return false in all cases except for Equal *)
-- apply false.
-- apply false.
-- apply false.
-(* Equal *)
-- destruct (do_computation user_functions e1 t).
-  (* lhs successfully computes *)
-  + destruct (do_computation user_functions e2 t).
-    (* rhs also successfully computes *)
-    { destruct t.
-      (* if t is tvProp, give up (no equality on Props!) *)
-      - apply false.
-      (* if t is an actual type, things get interesting.
-         we need to do some manipulation to get types to work out.
-         a naive approach would lead to Coq thinking that the implementation
-         pulled out of the types list, and the implementation from the tvarD
-         returned by do_computation don't match - but they do! *)
-      - unfold tvarD in *. unfold Impl_ in *.
-        destruct (nth_error all_types n).
-        (* if we found the type (we should have...) actually check equality *)
-        + apply (t.(Eqb) t0 t1).
-        (* otherwise, give up *)
-        + apply false.
-    }
-    (* rhs failed to compute *)
-    { apply false. }
-  (* lhs failed to compute *)
-  + apply false.
-(* the rest... *)
-- apply false.
-- apply false.
-Defined.
-
-
-(* some tests for do_compute_prop *)
-Eval vm_compute in (do_computation nil (Func 1 []) (tvType 11)).
-Eval vm_compute in (do_computation_equal nil (Equal (tvType 11) (Func 13 [(Func 1 [])]) (Func 13 [(Func 1 [])]))).
-
-Eval vm_compute in (do_computation nil (Func 13 [(Func 1 [])]) (tvType 11)).
-Eval vm_compute in (do_computation nil (Equal nat_tv (Func 1 []) (Func 1 [])) tvProp).
-Eval vm_compute in (do_computation nil (Equal nat_tv (Func 13 [(Func 1 [])]) (Func 1 [])) tvProp).
-Eval vm_compute in (do_computation nil (Equal nat_tv (Func 13 [(Func 1 [])]) (Func 13 [(Func 1 [])])) tvProp).
-
+  Proof.
+    intros.
+    simpl in H.
+    remember (do_computation user_functions r t) as do_rhs.
+    remember (do_computation user_functions l t) as do_lhs.
+    destruct do_lhs; destruct do_rhs; try (solve [inversion H]).
+    - consider (get_Eq all_types t t0 t1). intro.
+      exists t0. rewrite <- H. split; reflexivity.
+  Qed.
 
 End do_computation.
